Remove unused param of delocation predicate

theories/Coherence/AddAdd.v
@@ -3,7 +3,14 @@ Require Import Keep Drop Take Restrict SetOperations OUnion.
 
 Set Implicit Arguments.
 
+Definition ogetdef X (d:X) (o:option X) :=
+  match o with
+  | Some x => x
+  | None => d
+  end.
+
 Definition addAdd s := (fun (DL:set var) AP => mdo t <- AP; Some ((s ∩ DL) ∪ t)).
+Definition addAdd' s := (fun (DL:set var) AP => ((s ∩ DL) ∪ oget AP)).
 
 Lemma ifSndR_zip_addAdd s DL A B
  : length DL = length A
@@ -44,7 +51,20 @@ Proof.
     + eauto.
 Qed.
 
-Lemma PIR2_addAdds' s DL b c
+Lemma ifFstR_addAdds2 s A B C
+  : PIR2 Subset A C
+  -> PIR2 (ifFstR Subset) B C
+  -> PIR2 (ifFstR Subset) (zip (addAdd s) A B) C.
+Proof.
+  intros R1 R2.
+  general induction R1; inv R2; simpl; eauto using @PIR2.
+  + econstructor; eauto.
+    - inv pf0; simpl; econstructor.
+      * cset_tac; intuition.
+Qed.
+
+
+Lemma PIR2_addAdds3 s DL b c
   : length DL = length b
     -> PIR2 ≼ b c
     -> PIR2 ≼ b (zip (addAdd s) DL c).
@@ -59,14 +79,17 @@ Proof.
     + eauto.
 Qed.
 
-Lemma ifFstR_addAdds2 s A B C
-  : PIR2 Subset A C
-  -> PIR2 (ifFstR Subset) B C
-  -> PIR2 (ifFstR Subset) (zip (addAdd s) A B) C.
+Lemma PIR2_addAdds' s DL b c
+  : length DL = length b
+    -> PIR2 ≼ b c
+    -> PIR2 ≼ b (Some ⊝ zip (addAdd' s) DL c).
 Proof.
-  intros R1 R2.
-  general induction R1; inv R2; simpl; eauto using @PIR2.
-  + econstructor; eauto.
-    - inv pf0; simpl; econstructor.
-      * cset_tac; intuition.
+  intros. eapply length_length_eq in H.
+  general induction H; invt PIR2.
+  - econstructor.
+  - simpl. econstructor.
+    + destruct y,y0; simpl; try now econstructor.
+      * econstructor. inv pf. unfold addAdd'; simpl.
+        clear - H3; cset_tac.
+    + eauto.
 Qed.
