theories/Coherence/DelocationValidator.v
@@ -9,24 +9,23 @@ match goal with
   [ H : annotation _ _ |- annotation _ _ ] => inv H; eassumption
 end.
 
-Lemma trs_dec DL ZL s ans_lv ans
-  : {trs DL ZL s ans_lv ans} +
-    {~ trs DL ZL s ans_lv ans}.
+Lemma trs_dec DL s ans_lv ans
+  : {trs DL s ans_lv ans} +
+    {~ trs DL s ans_lv ans}.
 Proof.
-  revert DL ZL ans_lv ans.
+  revert DL ans_lv ans.
   sind s.
   time (destruct s; destruct ans; try solve [dec_right]; destruct ans_lv; try solve [dec_right]).
   + destruct a; [ | dec_right];
       destruct (IH s (ltac:(eauto))
-                   (restr (getAnn ans_lv \ singleton x) ⊝  DL) ZL ans_lv ans);
+                   (restr (getAnn ans_lv \ singleton x) ⊝  DL) ans_lv ans);
       [| dec_right].
     dec_solve.
   + destruct a; [| dec_right];
-    destruct (IH s1 (ltac:(eauto)) DL ZL ans_lv1 ans1); [| dec_right];
-    destruct (IH s2 (ltac:(eauto)) DL ZL ans_lv2 ans2); [| dec_right].
+    destruct (IH s1 (ltac:(eauto)) DL ans_lv1 ans1); [| dec_right];
+    destruct (IH s2 (ltac:(eauto)) DL ans_lv2 ans2); [| dec_right].
     dec_solve.
   + destruct (get_dec DL (counted l)) as [[[G'|]]|];[| dec_right | dec_right];
-    destruct (get_dec ZL (counted l)) as [[Za ?]|]; [| dec_right];
       destruct a; [| dec_right];
         dec_solve.
   + destruct a;[| dec_right].
@@ -35,12 +34,12 @@ Proof.
     ensure (length F = length sa);
     ensure(length F = length sa0).
     destruct (IH s (ltac:(eauto)) (Some ⊝ (getAnn ⊝ sa0) \\ app (A:=var) ⊜ (fst ⊝ F) a ++ DL)
-                 (a ++ ZL) ans_lv ans);[| dec_right].
+                 ans_lv ans);[| dec_right].
     edestruct (indexwise_R4_dec
                  (R:=fun lvs Zs Za' ans' =>
                        trs (restr (getAnn lvs \ of_list (fst Zs ++ Za'))
                                      ⊝ (Some ⊝ (getAnn ⊝ sa0) \\ app (A:=var) ⊜ (fst ⊝ F) a ++ DL))
-                           (a ++ ZL) (snd Zs) lvs ans')
+                           (snd Zs) lvs ans')
                  (LA:=sa0)
                  (LB:=F)
                  (LC:=a)
@@ -49,8 +48,8 @@ Proof.
     dec_solve. dec_right.
 Defined.
 
-Instance trs_dec_inst DL ZL s lv Y
-: Computable (trs DL ZL s lv Y).
+Instance trs_dec_inst DL s lv Y
+: Computable (trs DL s lv Y).
 Proof.
   hnf; eauto using trs_dec.
 Defined.
